+ lemma in low level

code/experimental/P256/Hacl.Impl.P256.LowLevel.fst
@@ -17,7 +17,7 @@ open FStar.Math.Lemmas
 
 open FStar.Mul
 
-#reset-options "--z3refresh --z3rlimit 100"
+#reset-options " --z3rlimit 300"
 
 
 inline_for_extraction
@@ -30,34 +30,50 @@ inline_for_extraction noextract
 val reduction_prime256_2prime256_with_carry_impl: cin: uint64 -> x: felem -> result: felem ->
   Stack unit 
     (requires fun h -> live h x /\ live h result /\  eq_or_disjoint x result /\ 
-      (let x = as_seq h x in  felem_seq_as_nat x + uint_v cin * pow2 256) < 2 * prime256)
+      (as_nat h x + uint_v cin * pow2 256) < 2 * prime256)
     (ensures fun h0 _ h1 -> modifies1 result h0 h1 /\ as_nat h1 result = (as_nat h0 x + uint_v cin * pow2 256) % prime256)  
 
 
 let reduction_prime256_2prime256_with_carry_impl cin x result = 
   push_frame();
     let tempBuffer = create (size 4) (u64 0) in 
-    let tempBufferForSubborrow = create (size 1) (u64 0) in 
+    let tempBufferForSubborrow = create (size 1) (u64 0) in
     recall_contents prime256_buffer (Lib.Sequence.of_list p256_prime_list);
     let c = sub4_il x prime256_buffer tempBuffer in
+  let h0 = ST.get() in 
+      assert(uint_v c <= 1);
+      assert(if uint_v c = 0 then as_nat h0 x >= prime256 else as_nat h0 x < prime256);
     let carry = sub_borrow c cin (u64 0) tempBufferForSubborrow in 
-      cmovznz4 carry tempBuffer x result;
-      let h3 = ST.get() in 
-      modulo_addition_lemma (felem_seq_as_nat (as_seq h3 result)) prime256 1;
-      small_modulo_lemma_1 (as_nat h3 result) prime256;
- pop_frame()   
+    cmovznz4 carry tempBuffer x result;
+  let h1 = ST.get() in 
+      assert_norm (pow2 64 * pow2 64 * pow2 64 * pow2 64 = pow2 256);
+      assert_norm (prime256 < pow2 256);
+      assert_norm(pow2 256 < 2 * prime256);
 
+      assert(uint_v cin <= 1);
+      assert(uint_v c <= 1);
 
-#reset-options "--z3rlimit 300"
+      assert(if as_nat h0 x >= prime256 then uint_v c = 0 else True);
+      assert(if uint_v cin < uint_v c then as_nat h1 result == as_nat h0 x else as_nat h1 result == as_nat h0 tempBuffer);
+
+      assert(as_nat h1 result < prime256);
+
+      modulo_addition_lemma (as_nat h1 result) prime256 1;
+      small_modulo_lemma_1 (as_nat h1 result) prime256; 
+  pop_frame()   
+
 
 inline_for_extraction
 val reduction_prime256_2prime256_8_with_carry_impl: x: widefelem -> result: felem -> 
   Stack unit 
     (requires fun h -> live h x /\ live h result /\ eq_or_disjoint x result /\ wide_as_nat h x < 2 * prime256)
-    (ensures fun h0 _ h1 -> modifies (loc result) h0 h1 /\ as_nat h1 result = (wide_as_nat h0 x) % prime256)
+    (ensures fun h0 _ h1 -> modifies (loc result) h0 h1 /\ as_nat h1 result = wide_as_nat h0 x % prime256)
 
 let reduction_prime256_2prime256_8_with_carry_impl x result = 
   push_frame();
+    assert_norm (pow2 64 * pow2 64 * pow2 64 * pow2 64 = pow2 256);
+    assert_norm (prime256 < pow2 256);
+    assert_norm(pow2 256 < 2 * prime256);
     let h0 = ST.get() in 
     let tempBuffer = create (size 4) (u64 0) in 
     let tempBufferForSubborrow = create (size 1) (u64 0) in 
@@ -80,18 +96,21 @@ let reduction_prime256_2prime256_8_with_carry_impl x result =
 	end );
  pop_frame()
 
+val lemma_reduction1_0: a: nat {a < pow2 256 /\ a >= prime256} -> r: nat{r = a - prime256} -> 
+  Lemma (r = a % prime256)
+
+let lemma_reduction1_0 a r = 
+  assert_norm (pow2 256 - prime256 < prime256);
+  small_modulo_lemma_1 r prime256; 
+  lemma_mod_sub_distr a prime256 prime256
+
 
 val lemma_reduction1: a: nat {a < pow2 256} -> r: nat{if a >= prime256 then r = a - prime256 else r = a} -> 
   Lemma (r = a % prime256)
 
 let lemma_reduction1 a r = 
-  assert_norm (pow2 256 - prime256 < prime256);
-  assert(if a >= prime256 then a - prime256 < prime256 else True);
-  assert(if a >= prime256 then r < prime256 else True);
-  assert(if a >= prime256 then r = a % prime256 else True);
-  assert(if a < prime256 then r < prime256 else True);
-  assert(if a < prime256 then r = a % prime256 else True);
-  assert(r = a % prime256)
+  if a >= prime256 then
+   lemma_reduction1_0 a r
 
 
 val reduction_prime_2prime_impl: x: felem -> result: felem -> 
