code/experimental/P256/Hacl.Spec.P256.Definitions.fst
@@ -199,17 +199,3 @@ let long_as_nat (h:mem) (e:long) : GTot nat =
   let s8 = s.[8] in 
   as_nat9 (s0, s1, s2, s3, s4, s5, s6, s7, s8)
 
-
-(* noextract
-let rec exp (e: nat) (n:nat {n > 0}) (prime: pos) : Tot (r: nat) (decreases n)  =
-  let ( *%) a b =  ( *% ) a b prime in 
-
-  if n = 1 then e
-  else
-    if n % 2 = 0 then 
-    begin
-      exp (e *% e) (n/2) prime
-    end
-    else e *% (exp (e *% e)((n-1)/2) prime) 
-*)
-
